TransVal/CombineEnv.v
@@ -1,0 +1,267 @@
+Require Import List Arith.
+Require Import IL Annotation AutoIndTac Bisim Exp MoreExp Coherence Fresh Util.
+Require Import SetOperations Sim Var.
+Require Import bitvec sexp smt nofun noGoto freeVars.
+Require Import Compute Guards ILFtoSMT tvalTactics TUtil GuardProps ComputeProps.
+
+(** Definitons **)
+Definition combineEnv D (E1:onv val) E2 :=
+fun x => if [x ∈ D] then E1 x else E2 x.
+
+(** Lemmata **)
+Lemma combineenv_agree D E E':
+  agree_on eq D (combineEnv D E E') E.
+
+Proof.
+  hnf; intros. unfold combineEnv. destruct if; eauto; isabsurd.
+Qed.
+
+Lemma exp_combineenv_eql:
+forall e D Es Et v,
+Exp.freeVars e ⊆ D
+-> (exp_eval (combineEnv D Es Et) e= v <-> exp_eval Es e = v).
+
+Proof.
+  intros. split; intros.
+  - eapply (exp_eval_agree (E:=(combineEnv D Es Et))); eauto.
+    eapply (agree_on_incl (bv:= Exp.freeVars e) (lv:= D));
+      cset_tac; eauto.
+    eapply combineenv_agree.
+  - eapply (exp_eval_agree (E:=Es)); eauto.
+    eapply (agree_on_incl (bv:=Exp.freeVars e) (lv:=D)); eauto.
+    symmetry. eapply combineenv_agree.
+Qed.
+
+  Lemma explist_combineenv_eql:
+forall el D Es Et rl,
+list_union (List.map Exp.freeVars el) ⊆ D
+-> ( omap (exp_eval (combineEnv D Es Et)) el = rl <-> omap (exp_eval Es) el = rl).
+
+Proof.
+  intros; split; intros.
+  - general induction el; eauto.
+    + simpl. simpl in H. hnf in H.
+      pose proof (exp_combineenv_eql a D Es Et (exp_eval (combineEnv D Es Et) a)); eauto.
+      destruct H0; hnf; intros; try setSubstUnion H.
+      * rewrite H0; eauto. erewrite IHel ; eauto.
+        hnf; intros. setSubstUnion H.
+  - general induction el; eauto.
+    + simpl; simpl in H; hnf in H;  unfold evalSexp.
+      pose proof (exp_combineenv_eql a D Es Et (exp_eval (combineEnv D Es Et) a)); eauto.
+      destruct H0; hnf; intros; try setSubstUnion H.
+      * rewrite H0; eauto. erewrite IHel; eauto.
+        hnf; intros; setSubstUnion H.
+Qed.
+
+Lemma combineenv_eql:
+forall F s D Es Et,
+ freeVars s ⊆  D
+->(  models F Es s  <-> models F (combineEnv D Es Et) s).
+
+Proof.
+  intros. eapply models_agree. eapply (agree_on_incl (lv:=D)); eauto; symmetry.
+  eapply combineenv_agree.
+Qed.
+
+Lemma exp_combineenv_eqr:
+forall e D Es Et v,
+agree_on eq (Exp.freeVars e ∩ D) Es Et
+-> (exp_eval (combineEnv D Es Et) e= v <-> exp_eval Et e = v).
+
+Proof.
+ intros; split; intros.
+ - eapply (exp_eval_agree (E:=(combineEnv D Es Et))); eauto.
+   hnf. cset_tac. unfold combineEnv. destruct if; eauto.
+   eapply H. cset_tac; intuition.
+ - eapply (exp_eval_agree (E:= Et)); eauto.
+   hnf; cset_tac. unfold combineEnv; destruct if; eauto.
+   symmetry. eapply H; cset_tac; intuition.
+Qed.
+
+Lemma explist_combineenv_eqr:
+forall el D Es Et vl,
+agree_on eq (list_union (List.map Exp.freeVars el) ∩ D) Es Et
+-> (omap (exp_eval (combineEnv D Es Et)) el = vl <-> omap (exp_eval Et) el = vl).
+
+Proof.
+  intros; split; intros.
+  - general induction el.
+    + reflexivity.
+    + simpl in *; hnf in H.
+      pose proof (exp_combineenv_eqr a D Es Et (exp_eval (combineEnv D Es Et) a)).
+      destruct H0.
+      * hnf; intros; cset_tac. eapply H. split; eauto.
+        unfold list_union; simpl. eapply list_union_start_swap; cset_tac; eauto.
+      * rewrite H0; eauto. f_equal.
+        rewrite (IHel D Es Et (omap (exp_eval (combineEnv D Es Et)) el)); eauto.
+        hnf. intros. cset_tac. eapply H. split; eauto.
+        unfold list_union. simpl. eapply list_union_start_swap. cset_tac; eauto.
+  - general induction el.
+    + reflexivity.
+    + simpl in *; hnf in H. unfold evalSexp.
+      pose proof (exp_combineenv_eqr a D Es Et (exp_eval Et a)).
+      destruct H0.
+      * hnf; intros; cset_tac. eapply H. split; eauto.
+        unfold list_union; simpl. eapply list_union_start_swap; cset_tac; eauto.
+      * rewrite H1; eauto. f_equal.
+        symmetry. rewrite (IHel D Es Et (omap (exp_eval  Et) el)); eauto.
+        hnf. intros. cset_tac. eapply H. split; eauto.
+        unfold list_union. simpl. eapply list_union_start_swap. cset_tac; eauto.
+Qed.
+
+Lemma combineenv_eqr:
+  forall  F s D Es Et,
+    agree_on eq (freeVars s ∩ D) Es Et
+    -> (models F Et s <-> models F (combineEnv D Es Et) s).
+
+Proof.
+  intros.  general induction s; try reflexivity; simpl.
+  - rewrite (IHs1 F D Es Et). rewrite (IHs2 F D Es Et).
+    + reflexivity.
+    + setSubst2 H.
+    + setSubst2 H.
+  - rewrite (IHs1 F D Es Et).  rewrite (IHs2 F D Es Et).
+    + reflexivity.
+    + setSubst2 H.
+    + setSubst2 H.
+  - rewrite (IHs F D Es Et).
+    + reflexivity.
+    + setSubst2 H.
+  -  unfold evalSexp.
+     case_eq (exp_eval (combineEnv D Es Et) e); intros.
+     + pose proof (exp_combineenv_eqr e D Es Et (Some v)).
+       assert (agree_on eq (Exp.freeVars e ∩ D) Es Et).
+       * hnf; intros. hnf in H. simpl in H. cset_tac. eapply H.
+         split; eauto.
+       * destruct H1; eauto.
+         specialize (H1 H0). rewrite H1.
+         case_eq (val2bool v); intros.
+         { rewrite (IHs1 F D Es Et).
+           - reflexivity.
+           - setSubst2 H. }
+         { rewrite (IHs2 F D Es Et).
+           - reflexivity.
+           - setSubst2 H. }
+     + pose proof (exp_combineenv_eqr e D Es Et None).
+       assert (agree_on eq (Exp.freeVars e ∩ D) Es Et).
+       * hnf; intros. hnf in H. simpl in H. cset_tac. eapply H.
+         split; eauto.
+       * destruct H1; eauto.  specialize (H1 H0). rewrite H1.
+         unfold default_val. simpl.
+         rewrite (IHs2 F D Es Et).
+         { reflexivity. }
+         { setSubst2 H. }
+  - rewrite (IHs1 F D Es Et).  rewrite (IHs2 F D Es Et).
+    + reflexivity.
+    + setSubst2 H.
+    + setSubst2 H.
+  - unfold evalSexp.
+    case_eq (exp_eval (combineEnv D Es Et) e); intros;
+    case_eq (exp_eval (combineEnv D Es Et) e0); intros.
+    + pose proof (exp_combineenv_eqr e D Es Et (Some v)).
+       assert (agree_on eq (Exp.freeVars e ∩ D) Es Et).
+       * hnf; intros. hnf in H. simpl in H. cset_tac. eapply H.
+         split; eauto.
+       * destruct H2; eauto. specialize (H2 H0). rewrite H2.
+         pose proof (exp_combineenv_eqr e0 D Es Et (Some v0)).
+         assert (agree_on eq (Exp.freeVars e0 ∩ D) Es Et).
+       { hnf; intros. hnf in H. simpl in H. cset_tac. eapply H.
+         split; eauto. }
+       { destruct H5; eauto. specialize (H5 H1). rewrite H5.
+         split; intros; eauto.
+       }
+    + pose proof (exp_combineenv_eqr e D Es Et (Some v)).
+      assert (agree_on eq (Exp.freeVars e ∩ D) Es Et).
+      * setSubst2 H.
+      * destruct H2; eauto. specialize (H2 H0). rewrite H2.
+        pose proof (exp_combineenv_eqr e0 D Es Et None).
+        assert (agree_on eq (Exp.freeVars e0 ∩ D) Es Et).
+        { setSubst2 H. }
+        { destruct H5; eauto. specialize (H5 H1). rewrite H5.
+          split; intros; eauto. }
+    + pose proof (exp_combineenv_eqr e D Es Et None).
+      assert (agree_on eq (Exp.freeVars e ∩ D) Es Et).
+      * setSubst2 H.
+      * destruct H2; eauto. specialize (H2 H0). rewrite H2.
+        pose proof (exp_combineenv_eqr e0 D Es Et (Some v)).
+        assert (agree_on eq (Exp.freeVars e0 ∩ D) Es Et).
+        { setSubst2 H. }
+        { destruct H5; eauto. specialize (H5 H1). rewrite H5.
+          split; intros; eauto. }
+    + pose proof (exp_combineenv_eqr e D Es Et None).
+      assert (agree_on eq (Exp.freeVars e ∩ D) Es Et).
+      * setSubst2 H.
+      * destruct H2; eauto. specialize (H2 H0). rewrite H2.
+        pose proof (exp_combineenv_eqr e0 D Es Et None).
+        assert (agree_on eq (Exp.freeVars e0 ∩ D) Es Et).
+        { setSubst2 H. }
+        { destruct H5; eauto.  specialize (H5 H1). rewrite H5.
+          split; intros; eauto. }
+  -unfold evalSpred; simpl. unfold labInc. destruct p.
+   unfold evalList.
+   pose proof (explist_combineenv_eqr a D Es Et (omap (exp_eval (combineEnv D Es Et)) a)).
+   destruct H0; eauto.
+   rewrite H0; eauto. reflexivity.
+  - unfold evalSpred. unfold evalSexp.
+    case_eq (exp_eval (combineEnv D Es Et) e); intros.
+    + pose proof (exp_combineenv_eqr e D Es Et (Some v)).
+      assert (agree_on eq (Exp.freeVars e ∩ D) Es Et).
+      * setSubst2 H.
+      * destruct H1; eauto.  specialize (H1 H0). rewrite H1.
+        split; intros; eauto.
+    + pose proof (exp_combineenv_eqr e D Es Et None).
+      assert (agree_on eq (Exp.freeVars e ∩ D) Es Et).
+      * setSubst2 H.
+      * destruct H1; eauto. specialize (H1 H0). rewrite H1.
+        split; intros; eauto.
+Qed.
+
+Lemma agree_on_ssa_combine:
+  forall D D' Ds' Dt' L E s t Es Et es et,
+    getAnn D = (Ds' ∩ Dt', Ds')
+    -> getAnn D' = (Ds' ∩ Dt', Dt')
+    -> ssa s D
+    -> ssa t D'
+    -> noFun s
+    -> noFun t
+    -> (forall x, x ∈ (Ds' ∩ Dt') -> exists v, E x = Some v)
+    ->Terminates (L, E, s) (L, Es, stmtReturn es)
+    -> Terminates (L, E, t) (L, Et, stmtReturn et)
+    -> (agree_on eq (Exp.freeVars et) Et (combineEnv Ds' Es Et)
+        /\ agree_on eq (Exp.freeVars es) Es (combineEnv Ds' Es Et)).
+
+Proof.
+  intros D D' Ds' Dt' L E s t Es Et es et.
+  intros getD getD' ssaS ssaT nfS nfT liveness sterm tterm.
+  split.
+  - pose proof (ssa_move_return D' L E t Et et nfT ssaT tterm).
+    destruct H as [D'' [ ssaRet [fstSubset sndSubset]]].
+    inv ssaRet.  rewrite getD' in *; simpl in *.
+    rewrite <- H1 in sndSubset.
+    hnf; intros.
+    unfold combineEnv.
+    destruct if; eauto.
+   + assert (x ∈ Ds' ∩ Dt').
+     * hnf in fstSubset. hnf in H0.  specialize (H0 x H).
+       cset_tac; eauto.
+     * specialize (liveness x  H2); destruct liveness.
+       pose proof (term_ssa_eval_agree L L s D (stmtReturn es) E Es ssaS nfS sterm).
+       pose proof (term_ssa_eval_agree L L t D' (stmtReturn et) E Et ssaT nfT tterm).
+       rewrite getD  in H4. rewrite getD'  in H5. simpl in *.
+       rewrite <- H4; eauto. rewrite <- H5; eauto.
+  - pose proof (ssa_move_return D L E s Es es nfS ssaS sterm).
+    destruct H as [D'' [ssaRet [fstSubset sndSubset]]].
+    inv ssaRet. rewrite getD in *; simpl in *.
+    rewrite <- H1 in sndSubset.
+    hnf; intros.
+    unfold combineEnv.
+    destruct if; eauto.
+    exfalso; apply n. hnf in H0. specialize (H0 x H).
+    eapply sndSubset; eauto.
+Qed.
+
+(*
+*** Local Variables: ***
+*** coq-load-path: (("../" "Lvc")) ***
+*** End: ***
+*)
