TransVal/freeVars.v
@@ -1,4 +1,5 @@
-Require Import List smt Exp Util CSet.
+Require Import List smt Exp Util CSet MapAgreement bitvec tvalTactics Val.
+Require Import OptionMap MoreExp.
 
 Fixpoint freeVars (s:smt) :=
 match s with
@@ -16,6 +17,43 @@ end.
 
 Definition freeVarsList el :=
 list_union (List.map freeVars el).
+
+Lemma models_agree F E E' s:
+  agree_on eq (freeVars s) E E'
+  -> (models F E s <-> models F E' s).
+
+Proof.
+intros agree; general  induction s; simpl in *; try reflexivity.
+- rewrite (IHs1 F E E'), (IHs2 F E E'); try reflexivity; setSubst2 agree.
+- rewrite (IHs1 F E E'), (IHs2 F E E'); try reflexivity; setSubst2 agree.
+- rewrite (IHs F E E'); try reflexivity; setSubst2 agree.
+- assert (agree_on eq (Exp.freeVars e) E E') by setSubst2 agree.
+  assert (exp_eval E e = exp_eval E' e)
+  by( eapply exp_eval_agree; symmetry; eauto).
+  case_eq (exp_eval E e); intros; unfold evalSexp.
+  +  rewrite <- H0. rewrite H1. case_eq(val2bool v); intros.
+     * rewrite (IHs1 F E E'); try reflexivity; setSubst2 agree.
+     * rewrite (IHs2 F E E'); try reflexivity; setSubst2 agree.
+  + rewrite <- H0; rewrite H1; simpl.
+    rewrite (IHs2 F E E'); try reflexivity; setSubst2 agree.
+- rewrite (IHs1 F E E'), (IHs2 F E E'); try reflexivity; setSubst2 agree.
+-  assert (exp_eval E e = exp_eval E' e)
+    by ( eapply exp_eval_agree; symmetry; eauto; setSubst2 agree).
+  assert (exp_eval E e0 = exp_eval E' e0)
+    by (eapply exp_eval_agree; symmetry; eauto; setSubst2 agree).
+  unfold evalSexp; rewrite <- H; rewrite <- H0.
+  unfold val2bool.
+  case_eq (exp_eval E e); case_eq (exp_eval E e0); intros;
+  rewrite bvEq_equiv_eq; reflexivity.
+- unfold evalSpred. destruct p.  unfold evalList.
+  assert (omap (exp_eval E) a = omap (exp_eval E')  a).
+  + eapply omap_exp_eval_agree; symmetry; eauto.
+  + rewrite <- H. destruct (omap (exp_eval E) a); reflexivity.
+- unfold evalSexp.
+  assert (exp_eval E e = exp_eval E' e)
+    by (eapply  exp_eval_agree; symmetry; eauto; setSubst2 agree).
+  rewrite <- H. case_eq (exp_eval E e); intros; reflexivity.
+Qed.
 
 (*
 *** Local Variables: ***
