TransVal/countAdmits.sh
@@ -1,0 +1,5 @@
+#!/bin/bash
+
+NUM=`grep "admit" $(find . -type f | grep -v '\.glob' | grep -v '\.sh') | wc -l`
+
+echo "There are $NUM admits left in the developement" | cowsay
